DynamoDbEncryption/src/DynamoDbEncryption/ConfigToInfo.dfy
@@ -6,31 +6,26 @@
 
   The only entry point of interest is 
 
-  Convert(outer : DynamoDbItemEncryptorConfig, config : Option<AwsCryptographyDynamoDbEncryptionTransformsTypes.SearchConfig>)
+  Convert(outer : DynamoDbTableEncryptionConfig, config : Option<AwsCryptographyDynamoDbEncryptionTransformsTypes.SearchConfig>)
     : Option<SearchableEncryptionInfo.SearchInfo>
   
   e.g. client.info :- Convert(config, config.beacons)
 */
 
 
-include "../../Model/AwsCryptographyDynamoDbEncryptionItemEncryptorTypes.dfy"
-include "../StructuredEncryption/SearchInfo.dfy"
 include "Util.dfy"
-include "../../Model/AwsCryptographyDynamoDbEncryptionTransformsTypes.dfy"
+include "SearchInfo.dfy"
 
 module SearchConfigToInfo {
-  import opened AwsCryptographyDynamoDbEncryptionItemEncryptorTypes
+  import opened AwsCryptographyDynamoDbEncryptionTypes
   import opened StandardLibrary
   import opened Wrappers
   import opened StandardLibrary.UInt
-  import opened DynamoDbItemEncryptorUtil
-  import C = AwsCryptographyDynamoDbEncryptionTypes
-  import DDBE = AwsCryptographyDynamoDbEncryptionTypes
+  import opened DynamoDbEncryptionUtil
+  import opened TermLoc
 
   import I = SearchableEncryptionInfo
-  import V = VirtualFields
-  import U = StructuredEncryptionUtil
-  import P = StructuredEncryptionPaths
+  import V = DdbVirtualFields
   import B = BaseBeacon
   import CB = CompoundBeacon
   import SE = AwsCryptographyStructuredEncryptionTypes
@@ -38,7 +33,7 @@ module SearchConfigToInfo {
   import Aws.Cryptography.Primitives
 
   // convert configured SearchConfig to internal SearchInfo
-  method Convert(outer : DynamoDbItemEncryptorConfig, config : Option<C.SearchConfig>)
+  method Convert(outer : DynamoDbTableEncryptionConfig, config : Option<SearchConfig>)
     returns (ret : Result<Option<I.SearchInfo>, Error>)
     ensures ret.Success? && ret.value.Some? ==>
       && ret.value.value.ValidState()
@@ -50,22 +45,21 @@ module SearchConfigToInfo {
       :- Need(|config.value.versions| == 1, E("search config must be have exactly one version."));
       var version :- ConvertVersion(outer, config.value.versions[0]);
       var info := I.SearchInfo(versions := [version], currWrite := 0);
-      var _ :- info.CheckValid()
-          .MapFailure(e => AwsCryptographyDynamoDbEncryption(DDBE.AwsCryptographyStructuredEncryption(e)));
+      var _ :- info.CheckValid();
       return Success(Some(info));
     }
   }
   
   // TODO : Placeholder
   function method GetPersistentKey(keyring: AwsCryptographyMaterialProvidersTypes.IKeyring)
-    : Result<U.Bytes, Error>
+    : Result<Bytes, Error>
   {
     Success([1,2,3,4,5])
   }
 
   // convert persistent key to the derived key for this beacon
-  method GetBeaconKey(client : Primitives.AtomicPrimitivesClient, key : U.Bytes, name : string)
-    returns (output : Result<U.Bytes, Error>)
+  method GetBeaconKey(client : Primitives.AtomicPrimitivesClient, key : Bytes, name : string)
+    returns (output : Result<Bytes, Error>)
     modifies client.Modifies
     requires client.ValidState()
     ensures client.ValidState()
@@ -82,7 +76,7 @@ module SearchConfigToInfo {
   }
 
   // convert configured BeaconVersion to internal BeaconVersion
-  method ConvertVersion(outer : DynamoDbItemEncryptorConfig, config : C.BeaconVersion)
+  method ConvertVersion(outer : DynamoDbTableEncryptionConfig, config : BeaconVersion)
     returns (output : Result<I.BeaconVersion, Error>)
   {
     :- Need(config.version == 1, E("Version number in BeaconVersion must be '1'."));
@@ -104,15 +98,9 @@ module SearchConfigToInfo {
     ));
   }
 
-  datatype VirtualField = | VirtualField (
-  nameonly name: string ,
-  nameonly config: string
-  )
-  type VirtualFieldList = seq<VirtualField>
-
   // convert configured VirtualFieldList to internal VirtualFieldMap
-  function method ConvertVirtualFields(outer : DynamoDbItemEncryptorConfig, vf : Option<VirtualFieldList>)
-    : Result<I.VirtualFieldMap, Error>
+  function method ConvertVirtualFields(outer : DynamoDbTableEncryptionConfig, vf : Option<VirtualFieldList>)
+    : Result<V.VirtualFieldMap, Error>
   {
     if vf.None? then
       Success(map[])
@@ -121,38 +109,38 @@ module SearchConfigToInfo {
   }
 
   // is this terminal location signed
-  predicate method IsSigned(outer : DynamoDbItemEncryptorConfig, loc : P.TerminalLocation)
+  predicate method IsSigned(outer : DynamoDbTableEncryptionConfig, loc : TermLoc)
   {
-    && var name := loc.parts[0].key;
+    && var name := loc[0].key;
     && name in outer.attributeActions
     && outer.attributeActions[name] != SE.DO_NOTHING
   }
 
   // is this terminal location encrypted
-  predicate method IsEncrypted(outer : DynamoDbItemEncryptorConfig, loc : P.TerminalLocation)
+  predicate method IsEncrypted(outer : DynamoDbTableEncryptionConfig, loc : TermLoc)
   {
-    && var name := loc.parts[0].key;
+    && var name := loc[0].key;
     && name in outer.attributeActions
     && outer.attributeActions[name] != SE.DO_NOTHING
   }
 
   // is this terminal location encrypted, OR does it refer to an encrypted virtual field
-  predicate method IsEncryptedV(outer : DynamoDbItemEncryptorConfig, virtualFields : I.VirtualFieldMap, loc : P.TerminalLocation)
+  predicate method IsEncryptedV(outer : DynamoDbTableEncryptionConfig, virtualFields : V.VirtualFieldMap, loc : TermLoc)
   {
-    var name := loc.parts[0].key;
+    var name := loc[0].key;
     if name in outer.attributeActions then
       outer.attributeActions[name] != SE.ENCRYPT_AND_SIGN
     else if name in virtualFields then
       var vf := virtualFields[name];
       // A virtual field is encrypted if any part is encrypted
-      vf.examine((t : P.TerminalLocation) => IsEncrypted(outer, t))
+      vf.examine((t : TermLoc) => IsEncrypted(outer, t))
     else
       false
   }
 
 
   // does this name already exists as a configured attribute, or virtual field
-  function method CheckExists2(outer : DynamoDbItemEncryptorConfig, virtualFields : I.VirtualFieldMap, name : string, context : string)
+  function method CheckExists2(outer : DynamoDbTableEncryptionConfig, virtualFields : V.VirtualFieldMap, name : string, context : string)
     : Result<bool, Error>
   {
     var _ :- CheckExists(outer, name, context);
@@ -163,7 +151,7 @@ module SearchConfigToInfo {
   }
 
   // does this name already exists as a configured attribute
-  function method CheckExists(outer : DynamoDbItemEncryptorConfig, name : string, context : string)
+  function method CheckExists(outer : DynamoDbTableEncryptionConfig, name : string, context : string)
     : Result<bool, Error>
   {
     if name in outer.attributeActions then
@@ -172,7 +160,7 @@ module SearchConfigToInfo {
       Failure(E(name + " not allowed as a " + context + " because it is already an allowed unauthenticated attribute."))
     else if outer.allowedUnauthenticatedAttributePrefix.Some? && outer.allowedUnauthenticatedAttributePrefix.value <= name then
       Failure(E(name + " not allowed as a " + context + " because it begins with the allowed unauthenticated prefix."))
-    else if U.ReservedPrefix <= name then
+    else if ReservedPrefix <= name then
       Failure(E(name + " not allowed as a " + context + " because it begins with the reserved prefix."))
     else
       Success(true)
@@ -180,30 +168,30 @@ module SearchConfigToInfo {
 
   // convert configured VirtualFields to internal VirtualFields
   function method {:tailrecursion} AddVirtualFields(
-      vf : seq<VirtualField>,
-      outer : DynamoDbItemEncryptorConfig,
-      converted : I.VirtualFieldMap := map[])
-    : Result<I.VirtualFieldMap, Error>
+      vf : seq<AwsCryptographyDynamoDbEncryptionTypes.VirtualField>,
+      outer : DynamoDbTableEncryptionConfig,
+      converted : V.VirtualFieldMap := map[])
+    : Result<V.VirtualFieldMap, Error>
   {
     if |vf| == 0 then
       Success(converted)
     else
       :- Need(vf[0].name !in converted, E("Duplicate VirtualField name : " + vf[0].name));
       var _ :- CheckExists(outer, vf[0].name, "VirtualField");
-      var newField :- V.GetVirtualField(vf[0].name, vf[0].config).MapFailure(e => E(e));
+      var newField :- V.ParseVirtualFieldConfig(vf[0]);
       // need all parts signed
-      :- Need(!newField.examine((t : P.TerminalLocation) => !IsSigned(outer, t)),
+      :- Need(!newField.examine((t : TermLoc) => !IsSigned(outer, t)),
         E("VirtualField " + vf[0].name + " must be defined on signed fields."));
       AddVirtualFields(vf[1..], outer, converted[vf[0].name := newField])
   }
 
   // convert configured StandardBeacons to internal Beacons
   method {:tailrecursion} AddStandardBeacons(
-      beacons : seq<C.StandardBeacon>,
-      outer : DynamoDbItemEncryptorConfig,
-      key : U.Bytes,
+      beacons : seq<StandardBeacon>,
+      outer : DynamoDbTableEncryptionConfig,
+      key : Bytes,
       client: Primitives.AtomicPrimitivesClient,
-      virtualFields : I.VirtualFieldMap,
+      virtualFields : V.VirtualFieldMap,
       converted : I.BeaconMap := map[])
     returns (output : Result<I.BeaconMap, Error>)
     modifies client.Modifies
@@ -217,25 +205,23 @@ module SearchConfigToInfo {
     var _ :- CheckExists2(outer, virtualFields, beacons[0].name, "StandardBeacon");
     var newKey :- GetBeaconKey(client, key, beacons[0].name);
     var locString := if beacons[0].loc.Some? then beacons[0].loc.value else beacons[0].name;
-    var newBeacon :- B.MakeStandardBeacon(client, beacons[0].name, newKey, beacons[0].length as B.BeaconLength, locString)
-      .MapFailure(e => AwsCryptographyDynamoDbEncryption(DDBE.AwsCryptographyStructuredEncryption(e)));
+    var newBeacon :- B.MakeStandardBeacon(client, beacons[0].name, newKey, beacons[0].length as B.BeaconLength, locString);
     :- Need(IsEncryptedV(outer, virtualFields, newBeacon.loc), E("StandardBeacon " + beacons[0].name + " not defined on an encrypted field."));
     output := AddStandardBeacons(beacons[1..], outer, key, client, virtualFields, converted[beacons[0].name := I.Standard(newBeacon)]);
   }
 
   // optional location, defaults to name
   function method GetLoc(name : string, loc : Option<string>)
-    : Result<P.TerminalLocation, Error>
+    : Result<TermLoc, Error>
   {
     if loc.None? then
-      P.TermLocMap?(name)
-        .MapFailure(e => AwsCryptographyDynamoDbEncryption(DDBE.AwsCryptographyStructuredEncryption(e)))
+      Success(TermLocMap(name))
     else
-      V.MakeTerminalLocation(loc.value).MapFailure(e => E(e))
+      MakeTermLoc(loc.value)
   }
 
   // convert configured NonSensitivePart to internal BeaconPart
-  function method {:tailrecursion} AddNonSensitiveParts(parts : seq<C.NonSensitivePart>, origSize : nat := |parts|, converted : seq<CB.BeaconPart> := [])
+  function method {:tailrecursion} AddNonSensitiveParts(parts : seq<NonSensitivePart>, origSize : nat := |parts|, converted : seq<CB.BeaconPart> := [])
     : (ret : Result<seq<CB.BeaconPart>, Error>)
     requires origSize == |parts| + |converted|
     ensures ret.Success? ==> |ret.value| == origSize
@@ -249,7 +235,7 @@ module SearchConfigToInfo {
   }
 
   // convert configured SensitivePart to internal BeaconPart
-  function method AddSensitiveParts(parts : seq<C.SensitivePart>, origSize : nat, converted : seq<CB.BeaconPart>)
+  function method AddSensitiveParts(parts : seq<SensitivePart>, origSize : nat, converted : seq<CB.BeaconPart>)
     : (ret : Result<seq<CB.BeaconPart>, Error>)
     requires origSize == |parts| + |converted|
     ensures ret.Success? ==> |ret.value| == origSize
@@ -277,7 +263,7 @@ module SearchConfigToInfo {
   }
 
   // convert configured ConstructorParts to internal ConstructorParts
-  function method MakeConstructor2(c : seq<C.ConstructorPart>, parts : seq<CB.BeaconPart>, origSize : nat, converted : seq<CB.ConstructorPart> := [])
+  function method MakeConstructor2(c : seq<ConstructorPart>, parts : seq<CB.BeaconPart>, origSize : nat, converted : seq<CB.ConstructorPart> := [])
     : (ret : Result<seq<CB.ConstructorPart>, Error>)
     requires origSize == |c| + |converted|
     ensures ret.Success? ==> |ret.value| == origSize
@@ -291,7 +277,7 @@ module SearchConfigToInfo {
   }
 
   // convert configured Constructor to internal Constructor
-  function method MakeConstructor(c : C.Constructor, parts : seq<CB.BeaconPart>)
+  function method MakeConstructor(c : Constructor, parts : seq<CB.BeaconPart>)
     : (ret : Result<CB.Constructor, Error>)
     requires 0 < |c.parts|
     ensures ret.Success? ==>
@@ -302,7 +288,7 @@ module SearchConfigToInfo {
   }
   
   // convert configured Constructors to internal Constructors
-  function method AddConstructors2(constructors : seq<C.Constructor>, parts : seq<CB.BeaconPart>, origSize : nat, converted : seq<CB.Constructor> := [])
+  function method AddConstructors2(constructors : seq<Constructor>, parts : seq<CB.BeaconPart>, origSize : nat, converted : seq<CB.Constructor> := [])
     : (ret : Result<seq<CB.Constructor>, Error>)
     requires 0 < origSize
     requires origSize == |constructors| + |converted|
@@ -317,7 +303,7 @@ module SearchConfigToInfo {
   }
 
   // convert configured Constructors to internal Constructors
-  function method AddConstructors(constructors : Option<C.ConstructorList>, parts : seq<CB.BeaconPart>)
+  function method AddConstructors(constructors : Option<ConstructorList>, parts : seq<CB.BeaconPart>)
     : (ret : Result<seq<CB.Constructor>, Error>)
     requires 0 < |parts|
     requires constructors.Some? ==> 0 < |constructors.value|
@@ -333,11 +319,11 @@ module SearchConfigToInfo {
 
   // convert configured CompoundBeacons to internal BeaconMap
   method {:tailrecursion} AddCompoundBeacons(
-      beacons : seq<C.CompoundBeacon>,
-      outer : DynamoDbItemEncryptorConfig,
-      key : U.Bytes,
+      beacons : seq<CompoundBeacon>,
+      outer : DynamoDbTableEncryptionConfig,
+      key : Bytes,
       client: Primitives.AtomicPrimitivesClient,
-      virtualFields : I.VirtualFieldMap,
+      virtualFields : V.VirtualFieldMap,
       converted : I.BeaconMap := map[])
     returns (output : Result<I.BeaconMap, Error>)
     modifies client.Modifies
@@ -358,10 +344,14 @@ module SearchConfigToInfo {
     parts :- AddSensitiveParts(beacons[0].sensitive, |parts| + |beacons[0].sensitive|, parts);
     :- Need(beacons[0].constructors.None? || 0 < |beacons[0].constructors.value|, E("For beacon " + beacons[0].name + " an empty constructor list was supplied."));
     var constructors :- AddConstructors(beacons[0].constructors, parts);
+    var beaconName := BeaconPrefix + beacons[0].name;
+    :- Need(DDB.IsValid_AttributeName(beaconName), E(beaconName + " is not a valid attribute name."));
+
     var newBeacon := CB.CompoundBeacon(
       B.BeaconBase (
         client := client,
         name := beacons[0].name,
+        beaconName := beaconName,
         key := key
       ),
       beacons[0].split[0],
@@ -373,12 +363,12 @@ module SearchConfigToInfo {
 
   // convert configured Beacons to internal BeaconMap
   method ConvertBeacons(
-    outer : DynamoDbItemEncryptorConfig,
-    key : U.Bytes,
+    outer : DynamoDbTableEncryptionConfig,
+    key : Bytes,
     client: Primitives.AtomicPrimitivesClient,
-    virtualFields : I.VirtualFieldMap,
-    standard : Option<C.StandardBeaconList>,
-    compound : Option<C.CompoundBeaconList>)
+    virtualFields : V.VirtualFieldMap,
+    standard : Option<StandardBeaconList>,
+    compound : Option<CompoundBeaconList>)
     returns (output : Result<I.BeaconMap, Error>)
     modifies client.Modifies
     requires client.ValidState()
