DynamoDbEncryption/src/DynamoDbEncryption/UpdateExpr.dfy
@@ -1,7 +1,7 @@
 // Copyright Amazon.com Inc. or its affiliates. All Rights Reserved.
 // SPDX-License-Identifier: Apache-2.0
 
-include "../../Model/AwsCryptographyDynamoDbEncryptionItemEncryptorTypes.dfy"
+include "Util.dfy"
 
 module DynamoDbUpdateExpr {
   import opened Wrappers
